split the compiler
git-svn-id: https://projects.brucker.ch/hol-testgen/svn/HOL-TestGen/trunk/hol-testgen@10592 3260e6d1-4efc-4170-b0a7-36055960796d

src/compiler/OCL_compiler_printer.thy
@@ -3,7 +3,7 @@
  *                       for the OMG Standard.
  *                       http://www.brucker.ch/projects/hol-testgen/
  *
- * OCL_compiler_meta_oid.thy ---
+ * OCL_compiler_printer.thy ---
  * This file is part of HOL-TestGen.
  *
  * Copyright (c) 2013-2014 Universite Paris-Sud, France
@@ -43,29 +43,48 @@
 
 header{* Part ... *}
 
-theory OCL_compiler_meta_oid
-imports OCL_compiler_init
+theory  OCL_compiler_printer
+imports OCL_compiler_core
+        "meta/OCL_compiler_printer_META"
 begin
 
-section{* oid Meta-Model aka. AST definition of oid *}
+section{* Generation to Deep Form: OCaml *}
 
-subsection{* type definition *}
+subsection{* conclusion *}
 
-datatype internal_oid = Oid nat
-datatype internal_oids = Oids nat (* start *)
-                              nat (* oid for assoc (incremented from start) *)
-                              nat (* oid for inh (incremented from start) *)
+definition "List_iterM f l =
+  List.fold (\<lambda>x m. bind m (\<lambda> () \<Rightarrow> f x)) l (return ())"
 
-subsection{* Oid-Management *}
+context s_of
+begin
+definition "write_file ocl = (
+  let (l_thy, Sys_argv) = ocl_compiler_config.more ocl
+    ; (is_file, f_output) = case (D_file_out_path_dep ocl, Sys_argv)
+     of (Some (file_out, _), Some dir) \<Rightarrow>
+          let dir = To_string dir in
+          (True, \<lambda>f. bind (Sys_is_directory2 dir) (\<lambda> Sys_is_directory2_dir.
+                     out_file1 f (if Sys_is_directory2_dir then sprintf2 (STR ''%s/%s.thy'') dir (To_string file_out) else dir)))
+      | _ \<Rightarrow> (False, out_stand1) in
+  f_output
+    (\<lambda>fprintf1.
+      List_iterM (fprintf1 (STR ''%s
+''                                 ))
+        (bug_ocaml_extraction (let (ocl, l) =
+           fold_thy'
+             (\<lambda>f. f ())
+             (\<lambda>_ _. [])
+             (\<lambda>x acc1 acc2. (acc1, Cons x acc2))
+             l_thy
+             (ocl_compiler_config.truncate ocl, []) in
+         s_of_thy_list (ocl_compiler_config_more_map (\<lambda>_. is_file) ocl) (rev l)))))"
+end
 
-definition "oidInit = (\<lambda> Oid n \<Rightarrow> Oids n n n)"
+definition "write_file = s_of.write_file implode (ToNat integer_of_natural)"
 
-definition "oidSucAssoc = (\<lambda> Oids n1 n2 n3 \<Rightarrow> Oids n1 (Succ n2) (Succ n3))"
-definition "oidSucInh = (\<lambda> Oids n1 n2 n3 \<Rightarrow> Oids n1 n2 (Succ n3))"
-definition "oidGetAssoc = (\<lambda> Oids _ n _ \<Rightarrow> Oid n)"
-definition "oidGetInh = (\<lambda> Oids _ _ n \<Rightarrow> Oid n)"
+lemmas [code] =
+  (* def *)
+  s_of.write_file_def
 
-definition "oidReinitAll = (\<lambda>Oids n1 _ _ \<Rightarrow> Oids n1 n1 n1)"
-definition "oidReinitInh = (\<lambda>Oids n1 n2 _ \<Rightarrow> Oids n1 n2 n2)"
+  (* fun *)
 
 end
