examples/Employee_DesignModel_UMLPart_generator_shallow.thy
@@ -47,8 +47,8 @@ theory
   Employee_DesignModel_UMLPart_generator_shallow
 imports
   "../src/OCL_main"
-  "../src/OCL_compiler_static"
-  "../src/OCL_compiler_generator_dynamic"
+  "../src/compiler/OCL_compiler_static"
+  "../src/compiler/OCL_compiler_generator_dynamic"
 begin
 
 generation_syntax [ shallow (generation_semantics [ analysis ])
