src/compiler/meta/OCL_compiler_meta_Pure.thy
@@ -44,7 +44,7 @@
 header{* Part ... *}
 
 theory  OCL_compiler_meta_Pure
-imports OCL_compiler_init
+imports "../OCL_compiler_init"
 begin
 
 section{* Lambda_pure Meta-Model aka. AST definition of Lambda_pure *}
